Update

theories/Completeness_seg/WK_seg_completeness.v
@@ -9,33 +9,31 @@ Require Import CKH_export.
 Require Import kripke_export.
 Require Import general_seg_completeness.
 
-
-
 Section WK_completeness.
 
-Definition is_k5 := (fun x => k5 = x).
+Definition is_Nd := (fun x => Nd = x).
 
-Lemma CF_k5 Γ : k5_frame (CF is_k5 Γ).
+Lemma CF_Nd Γ : Nd_frame (CF is_Nd Γ).
 Proof.
 intros w Hw.
 assert (@head _ _ w = Clos Γ).
 { apply Extensionality_Ensembles ; split ; intros A HA ; unfold In, head in * ; cbn in *.
-  - apply (segInclClos is_k5) in HA ; auto.
-  - apply (segClosed is_k5) ; auto. eapply MP. apply EFQ.
+  - apply (segInclClos is_Nd) in HA ; auto.
+  - apply (segClosed is_Nd) ; auto. eapply MP. apply EFQ.
     eapply MP. apply Ax. right. reflexivity.
-    apply Id. apply (truth_lemma is_k5).
+    apply Id. apply (truth_lemma is_Nd).
     right ; auto.
-    intros v Hv. apply Hw in Hv. exists (cexpl is_k5 Γ). split ; auto.
+    intros v Hv. apply Hw in Hv. exists (cexpl is_Nd Γ). split ; auto.
     cbn ; auto. }
 apply cmreach_expl ; auto.
 unfold cmreach ; cbn. rewrite H. apply In_singleton.
 Qed.
 
 Theorem WK_Strong_Completeness : forall Γ φ,
-    loc_conseq k5_frame Γ φ -> WKH_prv Γ φ.
+    loc_conseq Nd_frame Γ φ -> WKH_prv Γ φ.
 Proof.
-apply Strong_Completeness with (FraP:= k5_frame) ; auto.
-apply CF_k5.
+apply Strong_Completeness with (FraP:= Nd_frame) ; auto.
+apply CF_Nd.
 Qed.
 
 End WK_completeness.
