theories/Completeness_segAB/general_segAB_completeness.v
@@ -8,8 +8,8 @@ Require Import im_syntax.
 Require Import CKH_export.
 Require Import kripke_export.
 
-Require Import Classical.
 
+Axiom LEM : forall P, P \/ ~ P.
 
 Section general_segAB_completeness.
 
@@ -18,7 +18,7 @@ Variable AdAx : form -> Prop.
 Variable FraP : frame -> Prop.
 Hypothesis corresp_AdAx_FraP : forall F, FraP F <-> (forall A, AdAx A -> fvalid F A).
 
-Definition AdAxk3 := fun x => AdAx x \/ (exists A B, (k3 A B) = x).
+Definition AdAxCd := fun x => AdAx x \/ (exists A B, (Cd A B) = x).
 
 
 (* We construct the ABsegments for our canonical model *)
@@ -28,13 +28,13 @@ Class ABsegment : Type :=
     tail : @Ensemble (@Ensemble form) ;
 
     (* head and tail are closed under deduction *)
-    segClosed : forall th, (th = head \/ tail th) -> closed AdAxk3 th ;
+    segClosed : forall th, (th = head \/ tail th) -> closed AdAxCd th ;
     (* head and tail of the ABsegment are quasi-prime *)
     segPrime : forall th, (th = head \/ tail th) -> prime th ;
 
     (* The ABsegment is A or B *)
-    segAorB : (forall th, Theory AdAxk3 th -> (tail th <-> (forall C, (head (☐ C) -> th C) /\ (th C -> head (⬦ C))))) (*A*) \/
-                    (forall th, Theory AdAxk3 th -> (tail th <-> (forall C, (head (☐ C) -> th C)))) (*B*) ;
+    segAorB : (forall th, Theory AdAxCd th -> (tail th <-> (forall C, (head (☐ C) -> th C) /\ (th C -> head (⬦ C))))) (*A*) \/
+                    (forall th, Theory AdAxCd th -> (tail th <-> (forall C, (head (☐ C) -> th C)))) (*B*) ;
   }.
 
 Lemma boxreflect : forall seg A, (@head seg) (☐ A) -> forall th, (@tail seg) th -> th A.
@@ -50,15 +50,15 @@ Lemma diamwitness : forall seg A, (@head seg) (⬦ A) -> exists th, (@tail seg) 
 Proof.
 intros. destruct segAorB.
 (* A *)
-- destruct (classic (head (⬦ ⊥))).
+- destruct (LEM (head (⬦ ⊥))).
   + exists AllForm. split. 2: unfold AllForm ; auto. apply H0. apply Theory_AllForm.
      intro C ; split ; intro HC.
      unfold AllForm ; auto. apply segClosed ; auto. eapply MP. eapply MP.
-     apply Ax ; left ; right ; eapply k2 ; reflexivity. apply Nec. apply EFQ. apply Id ; auto.
-  + assert (~ pair_extCKH_prv AdAxk3 (Union _ (fun x => exists B, head (Box B) /\ x = B) (Singleton _ A)) (fun y => exists B, y = B /\ ~ head (⬦ B))).
+     apply Ax ; left ; right ; eapply Kd ; reflexivity. apply Nec. apply EFQ. apply Id ; auto.
+  + assert (~ pair_extCKH_prv AdAxCd (Union _ (fun x => exists B, head (Box B) /\ x = B) (Singleton _ A)) (fun y => exists B, y = B /\ ~ head (⬦ B))).
      { intro. destruct H2 as (l & H2 & H3). destruct l.
      * apply H1. apply segClosed ; auto.
-       eapply MP. 2: apply Id ; exact H. eapply MP. apply Ax ; left ; right ; eapply k2 ; reflexivity.
+       eapply MP. 2: apply Id ; exact H. eapply MP. apply Ax ; left ; right ; eapply Kd ; reflexivity.
        apply extCKH_Deduction_Theorem in H3. apply K_rule in H3. apply (extCKH_monot _ _ _ H3).
        intros C HC. destruct HC as (D & (E & K2 & K3) & K1) ; subst ; auto.
      * remember (f :: l) as l'. apply extCKH_Deduction_Theorem in H3. apply K_rule in H3.
@@ -70,13 +70,13 @@ intros. destruct segAorB.
        apply EFQ. apply Id ; auto. apply segPrime ; auto.
        intros B HB. inversion HB ; subst. destruct H4. destruct H4 ; subst. destruct H4. destruct H4 ; subst ; auto.
        inversion H4 ; subst ; auto. subst ; intro H4 ; inversion H4.
-       apply Ax ; left ; right ; eapply k2 ; reflexivity. }
+       apply Ax ; left ; right ; eapply Kd ; reflexivity. }
    apply (Lindenbaum_pair _ AllForm) in H2.
    destruct H2 as (Δm & G0 & G1 & G2 & G3 & G4). exists Δm. split ; auto.
    apply H0. split ; [intros B HB ; apply G2 ; unfold AllForm ; auto | apply LEM_prime ; auto].
    left. apply Incl_Set_ClosSubform ; unfold In ; auto.
    intro C ; split ; intro HC. apply G0. left ; exists C ; split ; auto.
-   destruct (classic (head (⬦ C))) ; auto. exfalso. apply G4. exists [C]. split ; auto.
+   destruct (LEM (head (⬦ C))) ; auto. exfalso. apply G4. exists [C]. split ; auto.
    intros. exists C ; split ; auto. inversion H3 ; subst ; auto. inversion H4.
    cbn. eapply MP. apply Ax ; left;  left ; eapply IA3 ; reflexivity. apply Id ; auto.
    apply G0. right ; apply In_singleton.
@@ -97,7 +97,7 @@ Axiom ABsegment_prf_irrel : forall (s0 s1 : ABsegment),
 
 (* Exploding world of the canonical model. *)
 
-Lemma cexpl_segClosed : forall th, (th = AllForm \/ (Singleton _ AllForm) th) ->  closed AdAxk3 th.
+Lemma cexpl_segClosed : forall th, (th = AllForm \/ (Singleton _ AllForm) th) ->  closed AdAxCd th.
 Proof.
 intros. destruct H ; subst ; intros A HA ; auto. unfold AllForm ; auto.
 inversion H ; subst ; auto. unfold AllForm ; auto.
@@ -108,8 +108,8 @@ Proof.
 intros. destruct H ; subst ; intros A B H0 ; left ; unfold AllForm ; auto ; inversion H ; unfold AllForm ; auto.
 Qed.
 
-Lemma cexpl_segAorB : (forall th, Theory AdAxk3 th -> ((Singleton _ AllForm) th <-> (forall C, (AllForm (☐ C) -> th C) /\ (th C -> AllForm (⬦ C))))) \/
-                    (forall th, Theory AdAxk3 th -> ((Singleton _ AllForm) th <-> (forall C, (AllForm (☐ C) -> th C)))).
+Lemma cexpl_segAorB : (forall th, Theory AdAxCd th -> ((Singleton _ AllForm) th <-> (forall C, (AllForm (☐ C) -> th C) /\ (th C -> AllForm (⬦ C))))) \/
+                    (forall th, Theory AdAxCd th -> ((Singleton _ AllForm) th <-> (forall C, (AllForm (☐ C) -> th C)))).
 Proof.
 right. intros. split ; intros.
 - inversion H0 ; subst ; unfold AllForm ; auto.
@@ -219,7 +219,7 @@ Instance CF : frame :=
    Lindenbaum lemma. *)
 
 Lemma Lindenbaum_ABsegment ψ Δ :
-  ~ extCKH_prv AdAxk3 Δ ψ ->
+  ~ extCKH_prv AdAxCd Δ ψ ->
   exists w : ABsegment, Included _ Δ head /\ ~ In _ head ψ.
 Proof.
   intros H1.
@@ -227,7 +227,7 @@ Proof.
   assert (J1: Included _ Δ (Clos AllForm)). intros C HC. left ; apply Incl_Set_ClosSubform ; unfold In ; unfold AllForm ; auto.
   pose (Lindenbaum _ _ _ _ J0 J1 H1).
   destruct s as (Δm & H2 & H3 & H4 & H5 & H6).
-  pose (Build_ABsegment Δm (fun th => Theory AdAxk3 th /\ (forall C, (Δm (☐ C) -> th C) /\ (th C -> Δm (⬦ C))))); intros.
+  pose (Build_ABsegment Δm (fun th => Theory AdAxCd th /\ (forall C, (Δm (☐ C) -> th C) /\ (th C -> Δm (⬦ C))))); intros.
   eexists (a _ _ _) ; split ; auto. intro. apply H6. apply Id ; auto.
   Unshelve. all: intros ; auto.
   - destruct H ; subst ; auto. intros C HC ; apply H4 ; auto.
@@ -316,8 +316,8 @@ induction ψ ; intros s ; split ; intros H0 ; simpl ; try simpl in H0 ; auto.
   left. apply IHψ1 ; auto.
   right. apply IHψ2 ; auto.
 (* Imp ψ1 ψ2 *)
-- destruct (classic (head (ψ1 --> ψ2))) ; auto. exfalso.
-  assert (~ extCKH_prv AdAxk3 (Union _ head (Singleton _ ψ1)) ψ2).
+- destruct (LEM (head (ψ1 --> ψ2))) ; auto. exfalso.
+  assert (~ extCKH_prv AdAxCd (Union _ head (Singleton _ ψ1)) ψ2).
   intro. apply extCKH_Deduction_Theorem in H1. apply H. apply segClosed ; auto.
   assert (Included form (Union _ head (Singleton form ψ1)) (Clos AllForm)).
   intros A HA. left. apply Incl_Set_ClosSubform ; unfold In ; unfold AllForm ; auto.
@@ -330,11 +330,11 @@ induction ψ ; intros s ; split ; intros H0 ; simpl ; try simpl in H0 ; auto.
 - intros.
   apply IHψ1 in H1 ; auto. unfold cireach in H. apply H in H0.
   apply IHψ2 ; auto.
-  assert (extCKH_prv AdAxk3 head ψ2). eapply MP. apply Id ; exact H0.
+  assert (extCKH_prv AdAxCd head ψ2). eapply MP. apply Id ; exact H0.
   apply Id ; auto. apply segClosed ; auto.
 (* Box ψ *)
-- destruct (classic (head (☐ ψ))) ; auto. exfalso.
-  assert (~ extCKH_prv AdAxk3 (fun x => exists A, (@head s) (☐ A) /\ x = A) ψ).
+- destruct (LEM (head (☐ ψ))) ; auto. exfalso.
+  assert (~ extCKH_prv AdAxCd (fun x => exists A, (@head s) (☐ A) /\ x = A) ψ).
   intro. apply H. apply segClosed ; auto. apply K_rule in H1.
   apply (extCKH_monot _ _ _ H1). intros B HB. unfold In in *.
   destruct HB as (C & (D & HD0 & HD1) & HC) ; subst ; auto.
@@ -343,74 +343,74 @@ induction ψ ; intros s ; split ; intros H0 ; simpl ; try simpl in H0 ; auto.
   2: intros C HC ; unfold In ; left ; apply Incl_Set_ClosSubform ; unfold In ; unfold AllForm ; auto.
   destruct H1 as (Γ0 & J0 & J1 & J2 & J3 & J4).
   (* Need to create the B-tail of head. *)
-  assert (forall th : Ensemble form, th = head \/ (fun x => Theory AdAxk3 x /\ (forall C, head (☐ C) -> x C)) th -> closed AdAxk3 th).
+  assert (forall th : Ensemble form, th = head \/ (fun x => Theory AdAxCd x /\ (forall C, head (☐ C) -> x C)) th -> closed AdAxCd th).
   intros. destruct H1 ; subst ; auto. apply (@segClosed s) ; auto. destruct H1 ; destruct H1 ; auto.
-  assert (forall th : Ensemble form, th = head \/ (fun x => Theory AdAxk3 x /\ (forall C, head (☐ C) -> x C)) th -> prime th).
+  assert (forall th : Ensemble form, th = head \/ (fun x => Theory AdAxCd x /\ (forall C, head (☐ C) -> x C)) th -> prime th).
   intros. destruct H2 ; subst ; auto. eapply (@segPrime s) ; auto. destruct H2 ; destruct H2 ; auto.
-  assert ((forall th, Theory AdAxk3 th -> ((fun x => Theory AdAxk3 x /\ (forall C, head (☐ C) -> x C)) th <-> (forall C, (head (☐ C) -> th C) /\ (th C -> head (⬦ C))))) \/
-                    (forall th, Theory AdAxk3 th -> ((fun x => Theory AdAxk3 x /\ (forall C, head (☐ C) -> x C)) th <-> (forall C, (head (☐ C) -> th C))))).
+  assert ((forall th, Theory AdAxCd th -> ((fun x => Theory AdAxCd x /\ (forall C, head (☐ C) -> x C)) th <-> (forall C, (head (☐ C) -> th C) /\ (th C -> head (⬦ C))))) \/
+                    (forall th, Theory AdAxCd th -> ((fun x => Theory AdAxCd x /\ (forall C, head (☐ C) -> x C)) th <-> (forall C, (head (☐ C) -> th C))))).
   right. intros ; split ; intros ; auto. apply H4 ; auto.
-  pose (Build_ABsegment head (fun x => Theory AdAxk3 x /\ (forall C, head (☐ C) -> x C)) H1 H2 H3).
+  pose (Build_ABsegment head (fun x => Theory AdAxCd x /\ (forall C, head (☐ C) -> x C)) H1 H2 H3).
   assert (cireach s a). intros C HC ; auto.
   (* Need to create the B-tail of Γ0 *)
-  assert (forall th : Ensemble form, th = Γ0 \/ (fun x => Theory AdAxk3 x /\ (forall C, Γ0 (☐ C) -> x C)) th -> closed AdAxk3 th).
+  assert (forall th : Ensemble form, th = Γ0 \/ (fun x => Theory AdAxCd x /\ (forall C, Γ0 (☐ C) -> x C)) th -> closed AdAxCd th).
   intros. destruct H5 ; subst ; auto. intros A HA ; apply J2 ; auto. left ; apply Incl_Set_ClosSubform ; unfold In ; unfold AllForm ; auto.
   destruct H5 ; destruct H5 ; auto.
-  assert (forall th : Ensemble form, th = Γ0 \/ (fun x => Theory AdAxk3 x /\ (forall C, Γ0 (☐ C) -> x C)) th -> prime th).
+  assert (forall th : Ensemble form, th = Γ0 \/ (fun x => Theory AdAxCd x /\ (forall C, Γ0 (☐ C) -> x C)) th -> prime th).
   intros. destruct H6 ; subst ; auto. apply LEM_prime ; auto. destruct H6 ; destruct H6 ; auto.
-  assert ((forall th, Theory AdAxk3 th -> ((fun x => Theory AdAxk3 x /\ (forall C, Γ0 (☐ C) -> x C)) th <-> (forall C, (Γ0 (☐ C) -> th C) /\ (th C -> Γ0 (⬦ C))))) \/
-                    (forall th, Theory AdAxk3 th -> ((fun x => Theory AdAxk3 x /\ (forall C, Γ0 (☐ C) -> x C)) th <-> (forall C, (Γ0 (☐ C) -> th C))))).
+  assert ((forall th, Theory AdAxCd th -> ((fun x => Theory AdAxCd x /\ (forall C, Γ0 (☐ C) -> x C)) th <-> (forall C, (Γ0 (☐ C) -> th C) /\ (th C -> Γ0 (⬦ C))))) \/
+                    (forall th, Theory AdAxCd th -> ((fun x => Theory AdAxCd x /\ (forall C, Γ0 (☐ C) -> x C)) th <-> (forall C, (Γ0 (☐ C) -> th C))))).
   right. intros ; split ; intros ; auto. apply H8 ; auto.
-  pose (Build_ABsegment Γ0 (fun x => Theory AdAxk3 x /\ (forall C, Γ0 (☐ C) -> x C)) H5 H6 H7).
+  pose (Build_ABsegment Γ0 (fun x => Theory AdAxCd x /\ (forall C, Γ0 (☐ C) -> x C)) H5 H6 H7).
   apply H0 with (u:=a0) in H4. apply IHψ in H4 ; auto. apply J4. apply Id. auto.
   unfold cmreach. unfold tail. unfold head. cbn. repeat split ; auto. intros. apply J0. exists C ; split ; auto.
 - intros. apply IHψ ; auto. apply H in H0. pose (boxreflect _ _ H0). apply p ; auto.
 (* Diam ψ *)
-- destruct (classic (head (⬦ ψ))) ; auto. exfalso.
-  assert (forall th : Ensemble form, th = head \/ (fun x => Theory AdAxk3 x /\ (forall C, (head (☐ C) -> x C) /\ (x C -> head (⬦ C)))) th -> closed AdAxk3 th).
+- destruct (LEM (head (⬦ ψ))) ; auto. exfalso.
+  assert (forall th : Ensemble form, th = head \/ (fun x => Theory AdAxCd x /\ (forall C, (head (☐ C) -> x C) /\ (x C -> head (⬦ C)))) th -> closed AdAxCd th).
   intros. destruct H1 ; subst ; auto. apply (@segClosed s) ; auto. destruct H1 ; destruct H1 ; auto.
-  assert (forall th : Ensemble form, th = head \/ (fun x => Theory AdAxk3 x /\ (forall C, (head (☐ C) -> x C) /\ (x C -> head (⬦ C)))) th -> prime th).
+  assert (forall th : Ensemble form, th = head \/ (fun x => Theory AdAxCd x /\ (forall C, (head (☐ C) -> x C) /\ (x C -> head (⬦ C)))) th -> prime th).
   intros. destruct H2 ; subst ; auto. eapply (@segPrime s) ; auto. destruct H2 ; destruct H2 ; auto.
-  assert ((forall th, Theory AdAxk3 th -> ((fun x => Theory AdAxk3 x /\ (forall C, (head (☐ C) -> x C) /\ (x C -> head (⬦ C)))) th <-> (forall C, (head (☐ C) -> th C) /\ (th C -> head (⬦ C))))) \/
-                    (forall th, Theory AdAxk3 th -> ((fun x => Theory AdAxk3 x /\ (forall C, (head (☐ C) -> x C) /\ (x C -> head (⬦ C)))) th <-> (forall C, (head (☐ C) -> th C))))).
+  assert ((forall th, Theory AdAxCd th -> ((fun x => Theory AdAxCd x /\ (forall C, (head (☐ C) -> x C) /\ (x C -> head (⬦ C)))) th <-> (forall C, (head (☐ C) -> th C) /\ (th C -> head (⬦ C))))) \/
+                    (forall th, Theory AdAxCd th -> ((fun x => Theory AdAxCd x /\ (forall C, (head (☐ C) -> x C) /\ (x C -> head (⬦ C)))) th <-> (forall C, (head (☐ C) -> th C))))).
   left. intros ; split ; intros ; auto. apply H4 ; auto.
-  pose (Build_ABsegment head (fun x => Theory AdAxk3 x /\ (forall C, (head (☐ C) -> x C) /\ (x C -> head (⬦ C)))) H1 H2 H3).
+  pose (Build_ABsegment head (fun x => Theory AdAxCd x /\ (forall C, (head (☐ C) -> x C) /\ (x C -> head (⬦ C)))) H1 H2 H3).
   assert (cireach s a). intros C HC ; auto.
   apply H0 in H4. destruct H4. destruct H4. apply IHψ in H5.
   unfold head in H5. apply H4 in H5. auto.
 - intros. unfold cireach in H. apply H in H0.
   apply diamwitness in H0. destruct H0. destruct H0.
-  assert (forall th : Ensemble form, th = x \/ (fun y => Theory AdAxk3 y /\ (forall C, x (☐ C) -> y C)) th -> closed AdAxk3 th).
+  assert (forall th : Ensemble form, th = x \/ (fun y => Theory AdAxCd y /\ (forall C, x (☐ C) -> y C)) th -> closed AdAxCd th).
   intros. destruct H2 ; subst ; auto. apply (@segClosed  _ x) ; auto. inversion H2. intros C HC ; auto. apply H3 ; auto.
-  assert (forall th : Ensemble form, th = x \/ (fun y => Theory AdAxk3 y /\ (forall C, x (☐ C) -> y C)) th -> prime th).
+  assert (forall th : Ensemble form, th = x \/ (fun y => Theory AdAxCd y /\ (forall C, x (☐ C) -> y C)) th -> prime th).
   intros. destruct H3 ; subst ; auto. eapply (@segPrime _ x) ; auto. destruct H3 ; destruct H3 ; auto.
-  assert ((forall th, Theory AdAxk3 th -> ((fun y => Theory AdAxk3 y /\ (forall C, x (☐ C) -> y C)) th <-> (forall C, (x (☐ C) -> th C) /\ (th C -> x (⬦ C))))) \/
-                    (forall th, Theory AdAxk3 th -> ((fun y => Theory AdAxk3 y /\ (forall C, x (☐ C) -> y C)) th <-> (forall C, (x (☐ C) -> th C))))).
+  assert ((forall th, Theory AdAxCd th -> ((fun y => Theory AdAxCd y /\ (forall C, x (☐ C) -> y C)) th <-> (forall C, (x (☐ C) -> th C) /\ (th C -> x (⬦ C))))) \/
+                    (forall th, Theory AdAxCd th -> ((fun y => Theory AdAxCd y /\ (forall C, x (☐ C) -> y C)) th <-> (forall C, (x (☐ C) -> th C))))).
   right. intros ; split ; intros ; auto. apply H5 ; auto.
-  pose (Build_ABsegment x (fun y => Theory AdAxk3 y /\ (forall C, x (☐ C) -> y C)) H2 H3 H4).
+  pose (Build_ABsegment x (fun y => Theory AdAxCd y /\ (forall C, x (☐ C) -> y C)) H2 H3 H4).
   exists a. split ; auto. apply IHψ ; auto.
 Qed.
 
-(* The canonical frames satisfies the sufficient condition of the axiom k3. *)
+(* The canonical frames satisfies the sufficient condition of the axiom Cd. *)
 
-Lemma CF_suff_k3 : suff_k3_frame CF.
+Lemma CF_suff_Cd : suff_Cd_frame CF.
 Proof.
 intro x.
 (* We create the A-segment in the cluster of x (it could be x, but we want to make sure). *)
-assert (forall th : Ensemble form, th = (@head x) \/ (fun w => Theory AdAxk3 w /\ (forall C, ((@head x)  (☐ C) -> w C) /\ (w C -> (@head  x) (⬦ C)))) th -> closed AdAxk3 th).
+assert (forall th : Ensemble form, th = (@head x) \/ (fun w => Theory AdAxCd w /\ (forall C, ((@head x)  (☐ C) -> w C) /\ (w C -> (@head  x) (⬦ C)))) th -> closed AdAxCd th).
 intros. destruct H ; subst ; auto. apply (@segClosed  x) ; auto. destruct H ; destruct H ; auto.
-assert (forall th : Ensemble form, th = (@head  x) \/ (fun w => Theory AdAxk3 w /\ (forall C, ((@head  x)  (☐ C) -> w C) /\ (w C -> (@head  x) (⬦ C)))) th -> prime th).
+assert (forall th : Ensemble form, th = (@head  x) \/ (fun w => Theory AdAxCd w /\ (forall C, ((@head  x)  (☐ C) -> w C) /\ (w C -> (@head  x) (⬦ C)))) th -> prime th).
 intros. destruct H0 ; subst ; auto. eapply (@segPrime x) ; auto. destruct H0 ; destruct H0 ; auto.
-assert ((forall th, Theory AdAxk3 th -> ((fun w => Theory AdAxk3 w /\ (forall C, ((@head  x)  (☐ C) -> w C) /\ (w C -> (@head  x) (⬦ C)))) th <-> (forall C, ((@head  x) (☐ C) -> th C) /\ (th C -> (@head  x) (⬦ C))))) \/
-                  (forall th, Theory AdAxk3 th -> ((fun w => Theory AdAxk3 w /\ (forall C, ((@head  x)  (☐ C) -> w C) /\ (w C -> (@head  x) (⬦ C)))) th <-> (forall C, ((@head  x) (☐ C) -> th C))))).
+assert ((forall th, Theory AdAxCd th -> ((fun w => Theory AdAxCd w /\ (forall C, ((@head  x)  (☐ C) -> w C) /\ (w C -> (@head  x) (⬦ C)))) th <-> (forall C, ((@head  x) (☐ C) -> th C) /\ (th C -> (@head  x) (⬦ C))))) \/
+                  (forall th, Theory AdAxCd th -> ((fun w => Theory AdAxCd w /\ (forall C, ((@head  x)  (☐ C) -> w C) /\ (w C -> (@head  x) (⬦ C)))) th <-> (forall C, ((@head  x) (☐ C) -> th C))))).
 left. intros ; split ; intros ; auto. apply H2 ; auto.
 pose (Build_ABsegment _ _ H H0 H1).
 exists a. repeat split ; auto.
 - intros A HA ; auto.
 - intros y z ixy maz.
-  destruct (classic (mreachable y cexpl)) as [P | NP].
+  destruct (LEM (mreachable y cexpl)) as [P | NP].
   { exists cexpl. split ; auto. intros A HA. unfold In ; unfold head ; unfold cexpl ; unfold AllForm ; auto. }
-  { assert (~ pair_extCKH_prv AdAxk3 (Union _ (fun B => (@head  y) (☐ B)) (@head  z)) (fun B => ~ (@head  y) (⬦ B))).
+  { assert (~ pair_extCKH_prv AdAxCd (Union _ (fun B => (@head  y) (☐ B)) (@head  z)) (fun B => ~ (@head  y) (⬦ B))).
   { intro. destruct H2 as (l & G0 & G1). destruct (partial_finite _ _ _ _ G1) as (l0 & G2 & G3).
     apply prv_list_left_conj in G3. apply extCKH_Deduction_Theorem in G3. apply K_rule in G3.
     apply MP with (B:=(⬦ list_conj l0) --> (⬦list_disj l)) in G3.
@@ -429,144 +429,38 @@ exists a. repeat split ; auto.
     apply ixy. unfold In. assert ((@head  x) = (@head  a)). auto. cbn. rewrite H3.
     apply maz. apply (@segClosed a) ; auto. apply forall_list_conj. intros. apply Id ; auto. apply G2 in H4 ; auto.
     intros B HB ; unfold In in * ; unfold head in *. destruct HB as (C & F0 & F1) ; subst ; auto.
-    apply Ax ; left ; right ; eapply k2 ; reflexivity. }
+    apply Ax ; left ; right ; eapply Kd ; reflexivity. }
   apply Lindenbaum_pair with (Γ:=AllForm) in H2.
   2-3: intros C HC ; left ; apply Incl_Set_ClosSubform ; unfold In ; unfold AllForm ; auto.
   destruct H2 as (Γ0 & J0 & J1 & J2 & J3 & J4).
-  assert (forall th : Ensemble form, th = Γ0 \/ (fun w => Theory AdAxk3 w /\ (forall C, (Γ0  (☐ C) -> w C) /\ (w C -> Γ0 (⬦ C)))) th -> closed AdAxk3 th).
+  assert (forall th : Ensemble form, th = Γ0 \/ (fun w => Theory AdAxCd w /\ (forall C, (Γ0  (☐ C) -> w C) /\ (w C -> Γ0 (⬦ C)))) th -> closed AdAxCd th).
   intros. destruct H2 ; subst ; auto. intros B HB. apply J2 ; auto. left ; apply Incl_Set_ClosSubform ; unfold In ; unfold AllForm ; auto.
   destruct H2 ; destruct H2 ; auto.
-  assert (forall th : Ensemble form, th = Γ0 \/ (fun w => Theory AdAxk3 w /\ (forall C, (Γ0  (☐ C) -> w C) /\ (w C -> Γ0 (⬦ C)))) th -> prime th).
+  assert (forall th : Ensemble form, th = Γ0 \/ (fun w => Theory AdAxCd w /\ (forall C, (Γ0  (☐ C) -> w C) /\ (w C -> Γ0 (⬦ C)))) th -> prime th).
   intros. destruct H3 ; subst ; auto. apply LEM_prime ; auto. destruct H3 ; destruct H3 ; auto.
-  assert ((forall th, Theory AdAxk3 th -> ((fun w => Theory AdAxk3 w /\ (forall C, (Γ0  (☐ C) -> w C) /\ (w C -> Γ0 (⬦ C)))) th <-> (forall C, (Γ0 (☐ C) -> th C) /\ (th C -> Γ0 (⬦ C))))) \/
-                    (forall th, Theory AdAxk3 th -> ((fun w => Theory AdAxk3 w /\ (forall C, (Γ0 (☐ C) -> w C) /\ (w C -> Γ0 (⬦ C)))) th <-> (forall C, (Γ0 (☐ C) -> th C))))).
+  assert ((forall th, Theory AdAxCd th -> ((fun w => Theory AdAxCd w /\ (forall C, (Γ0  (☐ C) -> w C) /\ (w C -> Γ0 (⬦ C)))) th <-> (forall C, (Γ0 (☐ C) -> th C) /\ (th C -> Γ0 (⬦ C))))) \/
+                    (forall th, Theory AdAxCd th -> ((fun w => Theory AdAxCd w /\ (forall C, (Γ0 (☐ C) -> w C) /\ (w C -> Γ0 (⬦ C)))) th <-> (forall C, (Γ0 (☐ C) -> th C))))).
   left. intros ; split ; intros ; auto. destruct H5 ; auto.
   pose (Build_ABsegment _ _ H2 H3 H4).
   exists a0. repeat split.
   + unfold mreachable ; cbn. unfold cmreach ; cbn. auto. pose (@segAorB y). destruct o.
      apply H5 ; auto. split ; auto. intro C ; split ; intro HC ; auto. apply J0 ; left ; auto.
-     destruct (classic ((@head y) (⬦ C))) ; auto.
+     destruct (LEM ((@head y) (⬦ C))) ; auto.
      exfalso. apply J4. exists [C]. split ; intros. inversion H7 ; subst ; auto.
      cbn. eapply MP. apply Ax ; left ; left ; eapply IA3 ; reflexivity. apply Id. auto.
      apply H5 ; auto. split ; auto. intros C HC ; auto. apply J0 ; left ; auto.
   + intros B HB. unfold In in * ; unfold head in * ; cbn in *. apply J0 ; right ; auto. }
 Qed.
 
-Lemma CF_k3 : k3_frame CF.
+Lemma CF_Cd : Cd_frame CF.
 Proof.
-apply suff_impl_k3. apply CF_suff_k3.
+apply suff_impl_Cd. apply CF_suff_Cd.
 Qed.
-
-(* Lemma CF_k3 : k3_frame CF.
-Proof.
-intros x y z ixy ixz Hy Hz.
-(* y is a A-segment *)
-assert (yA: forall th : form -> Prop, Theory AdAxk3 th -> (@tail y) th <-> (forall C : form, ((@head y) (☐ C) -> th C) /\ (th C -> (@head y) (⬦ C)))).
-{ destruct (@segAorB y) ; auto. exfalso. apply Hy. exists expl. split ; auto. apply In_singleton. apply H ; auto. apply Theory_AllForm.
-  intros. unfold head ; unfold expl ; cbn ; unfold AllForm ; auto. }
-(* z is a A-segment *)
-assert (zA: forall th : form -> Prop, Theory AdAxk3 th -> (@tail z) th <-> (forall C : form, ((@head z) (☐ C) -> th C) /\ (th C -> (@head z) (⬦ C)))).
-{ destruct (@segAorB z) ; auto. exfalso. apply Hz. exists expl. split ; auto. apply In_singleton. apply H ; auto. apply Theory_AllForm.
-  intros. unfold head ; unfold expl ; cbn ; unfold AllForm ; auto. }
-(* We create the A-segment in the cluster of x (it could be x, but we want to make sure). *)
-assert (forall th : Ensemble form, th = (@head x) \/ (fun w => Theory AdAxk3 w /\ (forall C, ((@head x)  (☐ C) -> w C) /\ (w C -> (@head  x) (⬦ C)))) th -> closed AdAxk3 th).
-intros. destruct H ; subst ; auto. apply (@segClosed  x) ; auto. destruct H ; destruct H ; auto.
-assert (forall th : Ensemble form, th = (@head  x) \/ (fun w => Theory AdAxk3 w /\ (forall C, ((@head  x)  (☐ C) -> w C) /\ (w C -> (@head  x) (⬦ C)))) th -> prime th).
-intros. destruct H0 ; subst ; auto. eapply (@segPrime x) ; auto. destruct H0 ; destruct H0 ; auto.
-assert ((forall th, Theory AdAxk3 th -> ((fun w => Theory AdAxk3 w /\ (forall C, ((@head  x)  (☐ C) -> w C) /\ (w C -> (@head  x) (⬦ C)))) th <-> (forall C, ((@head  x) (☐ C) -> th C) /\ (th C -> (@head  x) (⬦ C))))) \/
-                  (forall th, Theory AdAxk3 th -> ((fun w => Theory AdAxk3 w /\ (forall C, ((@head  x)  (☐ C) -> w C) /\ (w C -> (@head  x) (⬦ C)))) th <-> (forall C, ((@head  x) (☐ C) -> th C))))).
-left. intros ; split ; intros ; auto. apply H2 ; auto.
-pose (Build_ABsegment _ _ H H0 H1).
-exists a. repeat split ; auto.
-- intros A HA ; auto.
-- intros A HA ; unfold In in *. destruct HA as (s0 & K0 & K1). inversion K0 ; subst.
-  assert (~ pair_extCKH_prv AdAxk3 (Union _ (fun B => (@head  y) (☐ B)) (@head  A)) (fun B => ~ (@head  y) (⬦ B))).
-  { intro. destruct H2 as (l & G0 & G1). destruct (partial_finite _ _ _ _ G1) as (l0 & G2 & G3).
-    apply prv_list_left_conj in G3. apply extCKH_Deduction_Theorem in G3. apply K_rule in G3.
-    apply MP with (B:=(⬦ list_conj l0) --> (⬦list_disj l)) in G3.
-    apply extCKH_monot with (Γ1:= (@head  y)) in G3. apply extCKH_Detachment_Theorem in G3.
-    apply extCKH_monot with (Γ1:= (@head  y)) in G3.
-    destruct l.
-    { cbn in G3. apply (@segClosed  y) in G3 ; auto. apply Hy. exists expl. split.
-      apply In_singleton. apply yA ; auto. unfold head. unfold expl ; cbn. apply Theory_AllForm.
-      intro C ; split ; unfold head ; cbn ;  intros HC. unfold AllForm ; auto.
-      apply (@segClosed  y) ; auto. eapply MP. eapply MP. apply Ax ; left ; right ; eapply k2 ; reflexivity.
-      apply Nec. apply EFQ. apply Id ; auto. }
-    { apply Diam_distrib_list_disj in G3. apply (@segClosed  y) in G3. apply prime_list_disj in G3 ; auto.
-      destruct G3 as (C & F0 & F1). destruct F0 ; subst. apply in_map_iff in H2. destruct H2 as (D & F2 & F3) ; subst.
-      apply G0 with D ; auto. apply G0 with f ; cbn ; auto. apply (@segClosed  y) ; auto. eapply MP.
-      apply EFQ. apply Id ; auto. intros D R Hor ; apply (@segPrime y) ; auto. auto. intro. inversion H2. }
-    intros B HB ; unfold In in * ; unfold head in *. inversion HB ; subst ; auto. inversion H2 ; subst.
-    apply ixy. unfold In. assert ((@head  x) = (@head  a)). auto. cbn. rewrite H3.
-    apply K1. apply (@segClosed  A) ; auto. apply forall_list_conj. intros. apply Id ; auto. apply G2 in H4 ; auto.
-    intros B HB ; unfold In in * ; unfold head in *. destruct HB as (C & F0 & F1) ; subst ; auto.
-    apply Ax ; left ; right ; eapply k2 ; reflexivity. }
-  apply Lindenbaum_pair with (Γ:=AllForm) in H2.
-  2-3: intros C HC ; left ; apply Incl_Set_ClosSubform ; unfold In ; unfold AllForm ; auto.
-  destruct H2 as (Γ0 & J0 & J1 & J2 & J3 & J4).
-  assert (forall th : Ensemble form, th = Γ0 \/ (fun w => Theory AdAxk3 w /\ (forall C, (Γ0  (☐ C) -> w C) /\ (w C -> Γ0 (⬦ C)))) th -> closed AdAxk3 th).
-  intros. destruct H2 ; subst ; auto. intros B HB. apply J2 ; auto. left ; apply Incl_Set_ClosSubform ; unfold In ; unfold AllForm ; auto.
-  destruct H2 ; destruct H2 ; auto.
-  assert (forall th : Ensemble form, th = Γ0 \/ (fun w => Theory AdAxk3 w /\ (forall C, (Γ0  (☐ C) -> w C) /\ (w C -> Γ0 (⬦ C)))) th -> prime th).
-  intros. destruct H3 ; subst ; auto. apply LEM_prime ; auto. destruct H3 ; destruct H3 ; auto.
-  assert ((forall th, Theory AdAxk3 th -> ((fun w => Theory AdAxk3 w /\ (forall C, (Γ0  (☐ C) -> w C) /\ (w C -> Γ0 (⬦ C)))) th <-> (forall C, (Γ0 (☐ C) -> th C) /\ (th C -> Γ0 (⬦ C))))) \/
-                    (forall th, Theory AdAxk3 th -> ((fun w => Theory AdAxk3 w /\ (forall C, (Γ0 (☐ C) -> w C) /\ (w C -> Γ0 (⬦ C)))) th <-> (forall C, (Γ0 (☐ C) -> th C))))).
-  left. intros ; split ; intros ; auto. destruct H5 ; auto.
-  pose (Build_ABsegment _ _ H2 H3 H4).
-  exists a0. repeat split.
-  + exists y ; split. apply In_singleton. unfold mreachable ; cbn. unfold cmreach ; cbn. auto.
-     apply yA. split ; auto. intro C ; split ; intro HC ; auto. apply J0 ; left ; auto.
-     destruct (classic ((@head y) (⬦ C))) ; auto.
-     exfalso. apply J4. exists [C]. split ; intros. inversion H6 ; subst ; auto.
-     cbn. eapply MP. apply Ax ; left ; left ; eapply IA3 ; reflexivity. apply Id. auto.
-  + intros B HB. unfold In in * ; unfold head in * ; cbn in *. apply J0 ; right ; auto.
-- intros A HA ; unfold In in *. destruct HA as (s0 & K0 & K1). inversion K0 ; subst.
-  assert (~ pair_extCKH_prv AdAxk3 (Union _ (fun B => (@head  z) (☐ B)) (@head  A)) (fun B => ~ (@head  z) (⬦ B))).
-  { intro. destruct H2 as (l & G0 & G1). destruct (partial_finite _ _ _ _ G1) as (l0 & G2 & G3).
-    apply prv_list_left_conj in G3. apply extCKH_Deduction_Theorem in G3. apply K_rule in G3.
-    apply MP with (B:=(⬦ list_conj l0) --> (⬦list_disj l)) in G3.
-    apply extCKH_monot with (Γ1:= (@head  z)) in G3. apply extCKH_Detachment_Theorem in G3.
-    apply extCKH_monot with (Γ1:= (@head  z)) in G3.
-    destruct l.
-    { cbn in G3. apply (@segClosed  z) in G3 ; auto. apply Hz. exists expl. split.
-      apply In_singleton. apply zA ; auto. unfold head. unfold expl ; cbn. apply Theory_AllForm.
-      intro C ; split ; unfold head ; cbn ;  intros HC. unfold AllForm ; auto.
-      apply (@segClosed  z) ; auto. eapply MP. eapply MP. apply Ax ; left ; right ; eapply k2 ; reflexivity.
-      apply Nec. apply EFQ. apply Id ; auto. }
-    { apply Diam_distrib_list_disj in G3. apply (@segClosed  z) in G3. apply prime_list_disj in G3 ; auto.
-      destruct G3 as (C & F0 & F1). destruct F0 ; subst. apply in_map_iff in H2. destruct H2 as (D & F2 & F3) ; subst.
-      apply G0 with D ; auto. apply G0 with f ; cbn ; auto. apply (@segClosed  z) ; auto. eapply MP.
-      apply EFQ. apply Id ; auto. intros D R Hor ; apply (@segPrime z) ; auto. auto. intro. inversion H2. }
-    intros B HB ; unfold In in * ; unfold head in *. inversion HB ; subst ; auto. inversion H2 ; subst.
-    apply ixz. unfold In. assert ((@head  x) = (@head  a)). auto. cbn. rewrite H3.
-    apply K1. apply (@segClosed  A) ; auto. apply forall_list_conj. intros. apply Id ; auto. apply G2 in H4 ; auto.
-    intros B HB ; unfold In in * ; unfold head in *. destruct HB as (C & F0 & F1) ; subst ; auto.
-    apply Ax ; left ; right ; eapply k2 ; reflexivity. }
-  apply Lindenbaum_pair with (Γ:=AllForm) in H2.
-  2-3: intros C HC ; left ; apply Incl_Set_ClosSubform ; unfold In ; unfold AllForm ; auto.
-  destruct H2 as (Γ0 & J0 & J1 & J2 & J3 & J4).
-  assert (forall th : Ensemble form, th = Γ0 \/ (fun w => Theory AdAxk3 w /\ (forall C, (Γ0  (☐ C) -> w C) /\ (w C -> Γ0 (⬦ C)))) th -> closed AdAxk3 th).
-  intros. destruct H2 ; subst ; auto. intros B HB. apply J2 ; auto. left ; apply Incl_Set_ClosSubform ; unfold In ; unfold AllForm ; auto.
-  destruct H2 ; destruct H2 ; auto.
-  assert (forall th : Ensemble form, th = Γ0 \/ (fun w => Theory AdAxk3 w /\ (forall C, (Γ0  (☐ C) -> w C) /\ (w C -> Γ0 (⬦ C)))) th -> prime th).
-  intros. destruct H3 ; subst ; auto. apply LEM_prime ; auto. destruct H3 ; destruct H3 ; auto.
-  assert ((forall th, Theory AdAxk3 th -> ((fun w => Theory AdAxk3 w /\ (forall C, (Γ0  (☐ C) -> w C) /\ (w C -> Γ0 (⬦ C)))) th <-> (forall C, (Γ0 (☐ C) -> th C) /\ (th C -> Γ0 (⬦ C))))) \/
-                    (forall th, Theory AdAxk3 th -> ((fun w => Theory AdAxk3 w /\ (forall C, (Γ0 (☐ C) -> w C) /\ (w C -> Γ0 (⬦ C)))) th <-> (forall C, (Γ0 (☐ C) -> th C))))).
-  left. intros ; split ; intros ; auto. destruct H5 ; auto.
-  pose (Build_ABsegment _ _ H2 H3 H4).
-  exists a0. repeat split.
-  + exists z ; split. apply In_singleton. unfold mreachable ; cbn. unfold cmreach ; cbn. auto.
-     apply zA. split ; auto. intro C ; split ; intro HC ; auto. apply J0 ; left ; auto.
-     destruct (classic ((@head z) (⬦ C))) ; auto.
-     exfalso. apply J4. exists [C]. split ; intros. inversion H6 ; subst ; auto.
-     cbn. eapply MP. apply Ax ; left ; left ; eapply IA3 ; reflexivity. apply Id. auto.
-  + intros B HB. unfold In in * ; unfold head in * ; cbn in *. apply J0 ; right ; auto.
-Qed. *)
 
 Hypothesis CF_FraP : FraP CF.
 
 Theorem QuasiCompleteness : forall Γ φ,
-    ~ extCKH_prv AdAxk3 Γ φ -> ~ loc_conseq FraP Γ φ.
+    ~ extCKH_prv AdAxCd Γ φ -> ~ loc_conseq FraP Γ φ.
 Proof.
 intros Γ φ D H.
 apply Lindenbaum_ABsegment in D ; auto.
@@ -576,10 +470,10 @@ apply H2. apply truth_lemma ; auto.
 Qed.
 
 Theorem Strong_Completeness : forall Γ φ,
-    loc_conseq FraP Γ φ -> extCKH_prv AdAxk3 Γ φ.
+    loc_conseq FraP Γ φ -> extCKH_prv AdAxCd Γ φ.
 Proof.
 intros Γ φ LC. pose (QuasiCompleteness Γ φ).
-destruct (classic (extCKH_prv AdAxk3 Γ φ)) ; auto. exfalso.
+destruct (LEM (extCKH_prv AdAxCd Γ φ)) ; auto. exfalso.
 apply n ; assumption.
 Qed.
 
