theories/Completeness_th/IK_th_completeness.v
@@ -11,9 +11,9 @@ Require Import general_th_completeness.
 
 Section IK_completeness.
 
-Definition is_k5 := (fun x => k5 = x).
+Definition is_Nd := (fun x => Nd = x).
 
-Lemma CF_k5 : k5_frame (CF is_k5).
+Lemma CF_Nd : Nd_frame (CF is_Nd).
 Proof.
 intros w Hw.
 apply cmreach_expl ; auto.
@@ -26,12 +26,12 @@ unfold cmreach ; cbn. split ; intros A HA.
 Qed.
 
 Theorem Strong_Completeness : forall Γ φ,
-    loc_conseq (fun F => k3_frame F /\ k4_frame F /\ k5_frame F) Γ φ -> IKH_prv Γ φ.
+    loc_conseq (fun F => Cd_frame F /\ Idb_frame F /\ Nd_frame F) Γ φ -> IKH_prv Γ φ.
 Proof.
-intros. apply more_AdAx_more_prv with (AdAxk34 is_k5).
+intros. apply more_AdAx_more_prv with (AdAxCdIdb is_Nd).
 - intros A HA. destruct HA ; auto.
-- apply Strong_Completeness with (FraP:= fun F => k3_frame F /\ k4_frame F /\ k5_frame F) ; auto.
-  repeat split ; auto. 1-2: apply CF_k34. apply CF_k5.
+- apply Strong_Completeness with (FraP:= fun F => Cd_frame F /\ Idb_frame F /\ Nd_frame F) ; auto.
+  repeat split ; auto. 1-2: apply CF_CdIdb. apply CF_Nd.
 Qed.
 
 End IK_completeness.
